LivenessValidators.v
@@ -1,5 +1,29 @@
 Require Import DecSolve IL Annotation Liveness LengthEq.
 
+Instance argsLive_dec Caller Callee Y Z
+      : Computable (argsLive Caller Callee Y Z).
+Proof.
+  decide(length Y = length Z).
+  eapply length_length_eq in e. general induction e.
+  left; econstructor. 
+  decide(y ∈ Callee <-> live_exp_sound x Caller);
+  edestruct (IHe Caller Callee); try dec_solve; try eassumption; try inv an; eauto; try tauto.
+  right; intro. eapply argsLive_length in H. congruence.
+Qed.
+
+(*TODO: generalize this, it might be useful *)
+Instance list_get_live_computable Y lv
+: Computable (forall n y, get Y n y -> live_exp_sound y lv).
+Proof.
+  hnf. general induction Y. 
+  - left; isabsurd.
+  - decide (live_exp_sound a lv).
+    + edestruct IHY. 
+      * left; intros. inv H; eauto using get.
+      * right; intros; eauto using get.
+    + right; eauto using get.
+Qed.
+
 Definition live_sound_dec Lv s slv (an:annotation s slv)
       : Computable (live_sound Lv s slv).
 Proof. 
@@ -9,15 +33,15 @@ Proof.
     decide (live_exp_sound e a); try dec_solve.
   + edestruct IHs1; try inv an; eauto;
     edestruct IHs2; try inv an; eauto;
-    decide (x ∈ a); 
+    decide (live_exp_sound e a); 
     decide (getAnn slv1 ⊆ a); 
     decide (getAnn slv2 ⊆ a);
     try dec_solve; try eassumption; try inv an; eauto.
   + destruct (get_dec Lv (counted l)) as [[[blv Z] ?]|?];
     try decide ((blv \ of_list Z) ⊆ a);
-    decide (of_list Y ⊆ a);
+    try decide (forall n y, get Y n y -> live_exp_sound y a);
     try decide (length Y = length Z); try dec_solve.
-  +  decide(x ∈ a); try dec_solve.
+  + decide(live_exp_sound e a); try dec_solve.
   + edestruct IHs1; eauto; try inv an; eauto;
     edestruct IHs2; eauto; try inv an; eauto;
     decide ((of_list Z) ⊆ getAnn slv1); 
@@ -25,7 +49,6 @@ Proof.
     decide (getAnn slv2 ⊆ a); try dec_solve.
     Grab Existential Variables. eassumption. eassumption.
 Defined.
-
 
 Instance live_sound_dec_inst Lv s slv `{Computable(annotation s slv)}
 : Computable (live_sound Lv s slv).
@@ -45,7 +68,7 @@ Proof.
 (*    decide (x ∉ getAnn slv -> a ⊆ getAnn slv\{{x}});*) try dec_solve. 
   + edestruct IHs1; try inv an; eauto;
     edestruct IHs2; try inv an; eauto;
-    decide (x ∈ a); 
+    decide (live_exp_sound e a); 
     decide (getAnn slv1 ⊆ a); 
     decide (getAnn slv2 ⊆ a);
     try dec_solve; try eassumption; try inv an; eauto.
@@ -53,7 +76,7 @@ Proof.
     try decide ((blv \ of_list Z) ⊆ a);
     try decide (argsLive a blv Y Z); try dec_solve.
     left. econstructor; eauto using argsLive_length.
-  + decide(x ∈ a); try dec_solve.
+  + decide(live_exp_sound e a); try dec_solve.
   + edestruct IHs1; eauto; try inv an; eauto;
     edestruct IHs2; eauto; try inv an; eauto;
     decide ((getAnn slv1 \ of_list Z) ⊆ a);
